Add disjointness and error case to fix verification of Record.read

src/tls/Record.fst
@@ -125,17 +125,14 @@ private type input_buffer = b: Buffer.buffer UInt8.t {Buffer.length b = v maxlen
 noeq abstract type input_state = | InputState:
   pos: ref (len:UInt32.t {len <=^ maxlen}) ->
   b: input_buffer {
+    Buffer.disjoint_ref_1 b pos /\
     Buffer.frameOf b = Mem.frameOf pos /\ 
     Buffer.length b = v maxlen} -> 
   input_state
 
-// type input_state = {
-//   pos: ref (len:UInt32.t {len <=^ maxlen});
-//   b: input_buffer }
-
 private let parseHeaderBuffer (b: Buffer.buffer UInt8.t {Buffer.length b = headerLength}) : ST parsed_header
   (requires (fun h0 -> Buffer.live h0 b))
-  (ensures (fun h0 hdr h1 -> modifies_none h0 h1 /\ hdr = parseHeader (Bytes.hide (Buffer.as_seq h0 b))))
+  (ensures (fun h0 hdr h1 -> h0 == h1 /\ hdr = parseHeader (Bytes.hide (Buffer.as_seq h0 b))))
 =
   // some margin for progress
   parseHeader (BufferBytes.to_bytes headerLength b)
@@ -154,23 +151,24 @@ abstract let input_inv h0 (s: input_state) =
 private unfold val waiting_len:  s: input_state -> ST UInt32.t
   (requires fun h0 -> input_inv h0 s)
   (ensures fun h0 len h1 -> 
-    modifies_none h0 h1 /\ 
+    h0 == h1 /\
     ( let pv = UInt32.v (sel h0 s.pos) in 
       let l = UInt32.v len in 
       ( if pv < headerLength 
         then pv + l = headerLength
         else 
         match parseHeader (Bytes.hide (Buffer.as_seq h0 (Buffer.sub s.b 0ul headerLen))) with
-        | Correct (_,_,length) -> pv + l == headerLength + length 
-        | _                    -> False)))
+        | Correct (_,_,length) -> pv + l == headerLength + length)))
 
-#set-options "--z3rlimit 20" //18-04-20 now required; why?
+#reset-options "--max_fuel 0 --max_ifuel 0 --using_facts_from '* -LowParse -Format'"
 let waiting_len s =
   if !s.pos <^ headerLen
   then headerLen -^ !s.pos
   else
-    match parseHeaderBuffer (Buffer.sub s.b 0ul headerLen) with
-    | Correct (_,_,length) -> headerLen +^ uint_to_t length -^ !s.pos
+    let Correct (_,_,length) = parseHeaderBuffer (Buffer.sub s.b 0ul headerLen) in
+    headerLen +^ uint_to_t length -^ !s.pos
+
+
 // TODO later, use a length-field accessor instead of a header parser
 
 val alloc_input_state: r:_ -> ST input_state 
@@ -192,12 +190,15 @@ type read_result =
       pv:protocolVersion ->
       b:bytes {length b <= max_TLSCiphertext_fragment_length} -> read_result
 
+// 2018.04.25 SZ:
+// I had to modify the post-condition to say `input_inv` is preserved only if
+// the result is not a ReadError.
+// We return a ReadError when the header is invalid, but we still advance s.pos.
+// We could preserver the invariant unconditionally if we advanced it only when
+// the header is valid.
 val read: Transport.t -> s: input_state -> ST read_result
-  (requires fun h0 -> 
-    input_inv h0 s)
-  (ensures fun h0 _ h1 -> 
-    input_inv h1 s
-    )
+  (requires fun h0 -> input_inv h0 s)
+  (ensures fun h0 r h1 -> ReadError? r \/ input_inv h1 s)
 //18-04-20 TODO modifies clause on a ref + a buffer
 // let r = Mem.frameOf s.pos in
 // Mem.modifies_one r h0 h1 
@@ -206,76 +207,73 @@ val read: Transport.t -> s: input_state -> ST read_result
 //   (Set.singleton (Heap.addr_of (HS.as_ref s.pos)))
 //   h0 h1)
 
-//18-04-20 TBC, how to speed up verification attempts?
-//#set-options "--z3rlimit 100 --detail_errors"
-#set-options "--admit_smt_queries true"
+#reset-options "--max_fuel 0 --max_ifuel 0 --using_facts_from '* -LowParse -Format' --z3rlimit 30"
 let rec read tcp s =
   let h0 = ST.get() in 
   let header = Buffer.sub s.b 0ul headerLen in 
   let p0 = !s.pos in
   let waiting = waiting_len s in
   let dest = Buffer.sub s.b p0 waiting in
-
-  let h0' = ST.get() in 
   let res = Transport.recv tcp dest waiting in
-  let h1 = ST.get() in 
+  let h1 = ST.get() in
+  Buffer.lemma_reveal_modifies_1 dest h0 h1;
   // framing, with two cases depending on the input state.
-  assert(Buffer.modifies_1 dest h0' h1); 
-  Buffer.lemma_intro_modifies_0 h0 h0'; //18-04-21 required? botched transitivity?
-  assume(Buffer.modifies_1 dest h0 h1); //18-04-21 why does the assert fail?? 
-  Buffer.lemma_reveal_modifies_1 dest h0 h1; 
-  assert(sel h1 s.pos = p0); 
-  assert(p0 <^ headerLen \/ Buffer.disjoint header dest); 
-  assume(p0 <^ headerLen \/ Buffer.as_seq h0 header == Buffer.as_seq h1 header); 
-  if res = -1l then 
+  //assert(p0 <^ headerLen \/ Buffer.disjoint header dest);
+  //assert(p0 <^ headerLen \/ Buffer.as_seq h0 header == Buffer.as_seq h1 header);
+  if res = -1l then
     ReadError (AD_internal_error, "Transport.recv")
-  else if res = 0l
-  then (
-    trace "WouldBlock"; 
-    ReadWouldBlock )
-  else (
+  else
+  if res = 0l
+  then ( trace "WouldBlock"; ReadWouldBlock )
+  else
+    begin
     let received = Int.Cast.int32_to_uint32 res in
-    assert(received <=^ waiting);
-    assert(p0 +^ waiting <=^ maxlen);
+    assert (received <=^ waiting);
+    assert (p0 +^ waiting <=^ maxlen);
     let p1 = p0 +^ received in 
     s.pos := p1;
-    let h2 = ST.get() in 
-    assert(p0 <^ headerLen \/ Buffer.as_seq h0 header == Buffer.as_seq h2 header);
+    //let h2 = ST.get() in
+    //assert(p0 <^ headerLen \/ Buffer.as_seq h0 header == Buffer.as_seq h2 header);
     if received <^ waiting
-    then (
+    then
       // partial read; we remain in the same logical state
       // we should probably return ReadWouldBlock instead when non-blocking
-      assert(input_inv h2 s);
-      read tcp s )
-    else (
+      read tcp s
+    else
+      begin
       if p1 = headerLen 
-      then (
+      then
+        begin
         // we have just buffered the record header
         match parseHeaderBuffer header with
         | Error e -> ReadError e
-        | Correct(ct,pv,length) ->
-          if length = 0 then (
+        | Correct(ct, pv, length) ->
+          if length = 0 then
+            begin
             // zero-length packet, a corner case possibly excluded by the RFC
             s.pos := 0ul;
-            let h3 = get() in 
-            assert(input_inv h3 s);
-            Received ct pv empty_bytes )
-          else (
-            assume(input_inv h2 s);
-            read tcp s ))
-      else (
+            Received ct pv empty_bytes
+            end
+          else read tcp s
+        end
+      else
+        begin
         // we have just buffered the whole record
         assert(headerLen <=^ p0); 
         let hdr = parseHeaderBuffer header in 
-        assert(Correct? hdr); //18-04-19 why do I need this? is it a new problem?
         match hdr with
-        | Correct(ct,pv,length) -> (
+        | Correct(ct, pv, length) ->
+          begin
           let len = UInt32.uint_to_t length in
           let b = Buffer.sub s.b headerLen len in
           let payload = BufferBytes.to_bytes length b in
           s.pos := 0ul;
-          Received ct pv payload )
-      )))
+          Received ct pv payload
+          end
+        end
+      end
+    end
+
 (*        
 //18-01-24 recheck async 
 //    if length fresh = 0 then
